AOT_axioms.thy
@@ -151,135 +151,201 @@ AOT_theorem p_identity_3:
 AOT_define AOT_nonidentical :: \<open>\<tau> \<Rightarrow> \<tau> \<Rightarrow> \<phi>\<close> (infixl "\<noteq>" 50)
   noneq_infix: \<open>\<tau> \<noteq> \<sigma> \<equiv>\<^sub>d\<^sub>f \<not>(\<tau> = \<sigma>)\<close>
 
-AOT_theorem pl_1: \<open>\<phi> \<rightarrow> (\<psi> \<rightarrow> \<phi>)\<close>
-  by (auto simp: AOT_sem_imp)
-AOT_theorem pl_2: \<open>(\<phi> \<rightarrow> (\<psi> \<rightarrow> \<chi>)) \<rightarrow> ((\<phi> \<rightarrow> \<psi>) \<rightarrow> (\<phi> \<rightarrow> \<chi>))\<close>
-  by (auto simp: AOT_sem_imp)
-AOT_theorem pl_3: \<open>(\<not>\<phi> \<rightarrow> \<not>\<psi>) \<rightarrow> ((\<not>\<phi> \<rightarrow> \<psi>) \<rightarrow> \<phi>)\<close>
-  by (auto simp: AOT_sem_imp AOT_sem_not)
+AOT_axiom pl_1: \<open>\<phi> \<rightarrow> (\<psi> \<rightarrow> \<phi>)\<close>
+  by (auto simp: AOT_sem_imp AOT_model_axiomI)
+AOT_axiom pl_2: \<open>(\<phi> \<rightarrow> (\<psi> \<rightarrow> \<chi>)) \<rightarrow> ((\<phi> \<rightarrow> \<psi>) \<rightarrow> (\<phi> \<rightarrow> \<chi>))\<close>
+  by (auto simp: AOT_sem_imp AOT_model_axiomI)
+AOT_axiom pl_3: \<open>(\<not>\<phi> \<rightarrow> \<not>\<psi>) \<rightarrow> ((\<not>\<phi> \<rightarrow> \<psi>) \<rightarrow> \<phi>)\<close>
+  by (auto simp: AOT_sem_imp AOT_sem_not AOT_model_axiomI)
 
-AOT_theorem cqt_1: \<open>\<forall>\<alpha> \<phi>{\<alpha>} \<rightarrow> (\<tau>\<down> \<rightarrow> \<phi>{\<tau>})\<close>
-  by (auto simp: AOT_sem_denotes AOT_sem_forall AOT_sem_imp)
+AOT_axiom cqt_1: \<open>\<forall>\<alpha> \<phi>{\<alpha>} \<rightarrow> (\<tau>\<down> \<rightarrow> \<phi>{\<tau>})\<close>
+  by (auto simp: AOT_sem_denotes AOT_sem_forall AOT_sem_imp AOT_model_axiomI)
 
-AOT_theorem cqt_2_const_var: \<open>\<alpha>\<down>\<close> using AOT_sem_vars_denote .
-AOT_theorem cqt_2_lambda:
+AOT_axiom cqt_2_const_var: \<open>\<alpha>\<down>\<close> using AOT_sem_vars_denote by (rule AOT_model_axiomI)
+AOT_axiom cqt_2_lambda:
   assumes \<open>INSTANCE_OF_CQT_2(\<phi>)\<close>
   shows \<open>[\<lambda>\<nu>\<^sub>1...\<nu>\<^sub>n \<phi>{\<nu>\<^sub>1...\<nu>\<^sub>n}]\<down>\<close>
-  using assms by (simp add: AOT_sem_denotes AOT_instance_of_cqt_2_def)
-AOT_theorem cqt_2_lambda0:
+  using assms by (simp add: AOT_sem_denotes AOT_instance_of_cqt_2_def AOT_model_axiomI)
+AOT_axiom cqt_2_lambda0:
   shows \<open>[\<lambda> \<phi>]\<down>\<close>
+  apply (rule AOT_model_axiomI)
   using AOT_model_equiv_def AOT_sem_lambda_denotes existence_3 by fastforce
 
-AOT_theorem cqt_3: \<open>\<forall>\<alpha> (\<phi>{\<alpha>} \<rightarrow> \<psi>{\<alpha>}) \<rightarrow> (\<forall>\<alpha> \<phi>{\<alpha>} \<rightarrow> \<forall>\<alpha> \<psi>{\<alpha>})\<close>
-  by (simp add: AOT_sem_forall AOT_sem_imp)
-AOT_theorem cqt_4: \<open>\<phi> \<rightarrow> \<forall>\<alpha> \<phi>\<close>
-  by (simp add: AOT_sem_forall AOT_sem_imp)
-AOT_theorem cqt_5a: \<open>[\<Pi>]\<kappa>\<^sub>1...\<kappa>\<^sub>n \<rightarrow> (\<Pi>\<down> & \<kappa>\<^sub>1...\<kappa>\<^sub>n\<down>)\<close>
-  by (simp add: AOT_sem_conj AOT_sem_denotes AOT_sem_exe AOT_sem_imp)
-AOT_theorem cqt_5a_1: \<open>[\<Pi>]\<kappa> \<rightarrow> (\<Pi>\<down> & \<kappa>\<down>)\<close>
-  using cqt_5a by blast
-AOT_theorem cqt_5a_2: \<open>[\<Pi>]\<kappa>\<^sub>1\<kappa>\<^sub>2 \<rightarrow> (\<Pi>\<down> & \<kappa>\<^sub>1\<down> & \<kappa>\<^sub>2\<down>)\<close>
-  by (metis AOT_model_denotes_prod_def AOT_sem_conj AOT_sem_denotes AOT_sem_exe AOT_sem_imp case_prodD)
-AOT_theorem cqt_5a_3: \<open>[\<Pi>]\<kappa>\<^sub>1\<kappa>\<^sub>2\<kappa>\<^sub>3 \<rightarrow> (\<Pi>\<down> & \<kappa>\<^sub>1\<down> & \<kappa>\<^sub>2\<down> & \<kappa>\<^sub>3\<down>)\<close>
-  by (metis AOT_model_denotes_prod_def AOT_sem_conj AOT_sem_denotes AOT_sem_exe AOT_sem_imp case_prodD)
-AOT_theorem cqt_5a_4: \<open>[\<Pi>]\<kappa>\<^sub>1\<kappa>\<^sub>2\<kappa>\<^sub>3\<kappa>\<^sub>4 \<rightarrow> (\<Pi>\<down> & \<kappa>\<^sub>1\<down> & \<kappa>\<^sub>2\<down> & \<kappa>\<^sub>3\<down> & \<kappa>\<^sub>4\<down>)\<close>
-  by (metis AOT_model_denotes_prod_def AOT_sem_conj AOT_sem_denotes AOT_sem_exe AOT_sem_imp case_prodD)
-AOT_theorem cqt_5b: \<open>\<kappa>\<^sub>1...\<kappa>\<^sub>n[\<Pi>] \<rightarrow> (\<Pi>\<down> & \<kappa>\<^sub>1...\<kappa>\<^sub>n\<down>)\<close>
-  using AOT_sem_enc_denotes
-  by (auto simp: AOT_sem_conj AOT_sem_denotes AOT_sem_imp)
-AOT_theorem cqt_5b_1: \<open>\<kappa>[\<Pi>] \<rightarrow> (\<Pi>\<down> & \<kappa>\<down>)\<close>
-  using cqt_5b by blast
-AOT_theorem cqt_5b_2: \<open>\<kappa>\<^sub>1\<kappa>\<^sub>2[\<Pi>] \<rightarrow> (\<Pi>\<down> & \<kappa>\<^sub>1\<down> & \<kappa>\<^sub>2\<down>)\<close>
-  by (metis AOT_model_denotes_prod_def AOT_sem_conj AOT_sem_denotes AOT_sem_enc_denotes AOT_sem_imp case_prodD)
-AOT_theorem cqt_5b_3: \<open>\<kappa>\<^sub>1\<kappa>\<^sub>2\<kappa>\<^sub>3[\<Pi>] \<rightarrow> (\<Pi>\<down> & \<kappa>\<^sub>1\<down> & \<kappa>\<^sub>2\<down> & \<kappa>\<^sub>3\<down>)\<close>
-  by (metis AOT_model_denotes_prod_def AOT_sem_conj AOT_sem_denotes AOT_sem_enc_denotes AOT_sem_imp case_prodD)
-AOT_theorem cqt_5b_4: \<open>\<kappa>\<^sub>1\<kappa>\<^sub>2\<kappa>\<^sub>3\<kappa>\<^sub>4[\<Pi>] \<rightarrow> (\<Pi>\<down> & \<kappa>\<^sub>1\<down> & \<kappa>\<^sub>2\<down> & \<kappa>\<^sub>3\<down> & \<kappa>\<^sub>4\<down>)\<close>
-  by (metis AOT_model_denotes_prod_def AOT_sem_conj AOT_sem_denotes AOT_sem_enc_denotes AOT_sem_imp case_prodD)
+AOT_axiom cqt_3: \<open>\<forall>\<alpha> (\<phi>{\<alpha>} \<rightarrow> \<psi>{\<alpha>}) \<rightarrow> (\<forall>\<alpha> \<phi>{\<alpha>} \<rightarrow> \<forall>\<alpha> \<psi>{\<alpha>})\<close>
+  by (simp add: AOT_sem_forall AOT_sem_imp AOT_model_axiomI)
+AOT_axiom cqt_4: \<open>\<phi> \<rightarrow> \<forall>\<alpha> \<phi>\<close>
+  by (simp add: AOT_sem_forall AOT_sem_imp AOT_model_axiomI)
+AOT_axiom cqt_5a: \<open>[\<Pi>]\<kappa>\<^sub>1...\<kappa>\<^sub>n \<rightarrow> (\<Pi>\<down> & \<kappa>\<^sub>1...\<kappa>\<^sub>n\<down>)\<close>
+  by (simp add: AOT_sem_conj AOT_sem_denotes AOT_sem_exe AOT_sem_imp AOT_model_axiomI)
+AOT_axiom cqt_5a_1: \<open>[\<Pi>]\<kappa> \<rightarrow> (\<Pi>\<down> & \<kappa>\<down>)\<close>
+  using cqt_5a AOT_model_axiomI by blast
+AOT_axiom cqt_5a_2: \<open>[\<Pi>]\<kappa>\<^sub>1\<kappa>\<^sub>2 \<rightarrow> (\<Pi>\<down> & \<kappa>\<^sub>1\<down> & \<kappa>\<^sub>2\<down>)\<close>
+  by (rule AOT_model_axiomI)
+     (metis AOT_model_denotes_prod_def AOT_sem_conj AOT_sem_denotes AOT_sem_exe AOT_sem_imp case_prodD)
+AOT_axiom cqt_5a_3: \<open>[\<Pi>]\<kappa>\<^sub>1\<kappa>\<^sub>2\<kappa>\<^sub>3 \<rightarrow> (\<Pi>\<down> & \<kappa>\<^sub>1\<down> & \<kappa>\<^sub>2\<down> & \<kappa>\<^sub>3\<down>)\<close>
+  by (rule AOT_model_axiomI)
+     (metis AOT_model_denotes_prod_def AOT_sem_conj AOT_sem_denotes AOT_sem_exe AOT_sem_imp case_prodD)
+AOT_axiom cqt_5a_4: \<open>[\<Pi>]\<kappa>\<^sub>1\<kappa>\<^sub>2\<kappa>\<^sub>3\<kappa>\<^sub>4 \<rightarrow> (\<Pi>\<down> & \<kappa>\<^sub>1\<down> & \<kappa>\<^sub>2\<down> & \<kappa>\<^sub>3\<down> & \<kappa>\<^sub>4\<down>)\<close>
+  by (rule AOT_model_axiomI)
+     (metis AOT_model_denotes_prod_def AOT_sem_conj AOT_sem_denotes AOT_sem_exe AOT_sem_imp case_prodD)
+AOT_axiom cqt_5b: \<open>\<kappa>\<^sub>1...\<kappa>\<^sub>n[\<Pi>] \<rightarrow> (\<Pi>\<down> & \<kappa>\<^sub>1...\<kappa>\<^sub>n\<down>)\<close>
+  by (rule AOT_model_axiomI)
+     (insert AOT_sem_enc_denotes; auto simp: AOT_sem_conj AOT_sem_denotes AOT_sem_imp)
+AOT_axiom cqt_5b_1: \<open>\<kappa>[\<Pi>] \<rightarrow> (\<Pi>\<down> & \<kappa>\<down>)\<close>
+  using cqt_5b AOT_model_axiomI by blast
+AOT_axiom cqt_5b_2: \<open>\<kappa>\<^sub>1\<kappa>\<^sub>2[\<Pi>] \<rightarrow> (\<Pi>\<down> & \<kappa>\<^sub>1\<down> & \<kappa>\<^sub>2\<down>)\<close>
+  by (rule AOT_model_axiomI)
+     (metis AOT_model_denotes_prod_def AOT_sem_conj AOT_sem_denotes AOT_sem_enc_denotes AOT_sem_imp case_prodD)
+AOT_axiom cqt_5b_3: \<open>\<kappa>\<^sub>1\<kappa>\<^sub>2\<kappa>\<^sub>3[\<Pi>] \<rightarrow> (\<Pi>\<down> & \<kappa>\<^sub>1\<down> & \<kappa>\<^sub>2\<down> & \<kappa>\<^sub>3\<down>)\<close>
+  by (rule AOT_model_axiomI)
+     (metis AOT_model_denotes_prod_def AOT_sem_conj AOT_sem_denotes AOT_sem_enc_denotes AOT_sem_imp case_prodD)
+AOT_axiom cqt_5b_4: \<open>\<kappa>\<^sub>1\<kappa>\<^sub>2\<kappa>\<^sub>3\<kappa>\<^sub>4[\<Pi>] \<rightarrow> (\<Pi>\<down> & \<kappa>\<^sub>1\<down> & \<kappa>\<^sub>2\<down> & \<kappa>\<^sub>3\<down> & \<kappa>\<^sub>4\<down>)\<close>
+  by (rule AOT_model_axiomI)
+     (metis AOT_model_denotes_prod_def AOT_sem_conj AOT_sem_denotes AOT_sem_enc_denotes AOT_sem_imp case_prodD)
 
-AOT_theorem l_identity: \<open>\<alpha> = \<beta> \<rightarrow> (\<phi>{\<alpha>} \<rightarrow> \<phi>{\<beta>})\<close>
-  by (simp add: AOT_sem_eq AOT_sem_imp)
+AOT_axiom l_identity: \<open>\<alpha> = \<beta> \<rightarrow> (\<phi>{\<alpha>} \<rightarrow> \<phi>{\<beta>})\<close>
+  by (rule AOT_model_axiomI)
+     (simp add: AOT_sem_eq AOT_sem_imp)
 
-AOT_act_theorem logic_actual: \<open>\<^bold>\<A>\<phi> \<rightarrow> \<phi>\<close>
-  by (simp add: AOT_sem_act AOT_sem_imp)
+AOT_act_axiom logic_actual: \<open>\<^bold>\<A>\<phi> \<rightarrow> \<phi>\<close>
+  by (rule AOT_model_act_axiomI)
+     (simp add: AOT_sem_act AOT_sem_imp)
 
-AOT_theorem logic_actual_nec_1: \<open>\<^bold>\<A>\<not>\<phi> \<equiv> \<not>\<^bold>\<A>\<phi>\<close>
-  by (simp add: AOT_sem_act AOT_sem_equiv AOT_sem_not)
-AOT_theorem logic_actual_nec_2: \<open>\<^bold>\<A>(\<phi> \<rightarrow> \<psi>) \<equiv> (\<^bold>\<A>\<phi> \<rightarrow> \<^bold>\<A>\<psi>)\<close>
-  by (simp add: AOT_sem_act AOT_sem_equiv AOT_sem_imp)
+AOT_axiom logic_actual_nec_1: \<open>\<^bold>\<A>\<not>\<phi> \<equiv> \<not>\<^bold>\<A>\<phi>\<close>
+  by (rule AOT_model_axiomI)
+     (simp add: AOT_sem_act AOT_sem_equiv AOT_sem_not)
+AOT_axiom logic_actual_nec_2: \<open>\<^bold>\<A>(\<phi> \<rightarrow> \<psi>) \<equiv> (\<^bold>\<A>\<phi> \<rightarrow> \<^bold>\<A>\<psi>)\<close>
+  by (rule AOT_model_axiomI)
+     (simp add: AOT_sem_act AOT_sem_equiv AOT_sem_imp)
 
-AOT_theorem logic_actual_nec_3: \<open>\<^bold>\<A>(\<forall>\<alpha> \<phi>{\<alpha>}) \<equiv> \<forall>\<alpha> \<^bold>\<A>\<phi>{\<alpha>}\<close>
-  by (simp add: AOT_sem_act AOT_sem_equiv AOT_sem_forall AOT_sem_denotes)
-AOT_theorem logic_actual_nec_4: \<open>\<^bold>\<A>\<phi> \<equiv> \<^bold>\<A>\<^bold>\<A>\<phi>\<close>
-  by (simp add: AOT_sem_act AOT_sem_equiv)
+AOT_axiom logic_actual_nec_3: \<open>\<^bold>\<A>(\<forall>\<alpha> \<phi>{\<alpha>}) \<equiv> \<forall>\<alpha> \<^bold>\<A>\<phi>{\<alpha>}\<close>
+  by (rule AOT_model_axiomI)
+     (simp add: AOT_sem_act AOT_sem_equiv AOT_sem_forall AOT_sem_denotes)
+AOT_axiom logic_actual_nec_4: \<open>\<^bold>\<A>\<phi> \<equiv> \<^bold>\<A>\<^bold>\<A>\<phi>\<close>
+  by (rule AOT_model_axiomI)
+     (simp add: AOT_sem_act AOT_sem_equiv)
 
-AOT_theorem qml_1: \<open>\<box>(\<phi> \<rightarrow> \<psi>) \<rightarrow> (\<box>\<phi> \<rightarrow> \<box>\<psi>)\<close>
-  by (simp add: AOT_sem_box AOT_sem_imp)
-AOT_theorem qml_2: \<open>\<box>\<phi> \<rightarrow> \<phi>\<close>
-  by (simp add: AOT_sem_box AOT_sem_imp)
-AOT_theorem qml_3: \<open>\<diamond>\<phi> \<rightarrow> \<box>\<diamond>\<phi>\<close>
-  by (simp add: AOT_sem_box AOT_sem_dia AOT_sem_imp)
+AOT_axiom qml_1: \<open>\<box>(\<phi> \<rightarrow> \<psi>) \<rightarrow> (\<box>\<phi> \<rightarrow> \<box>\<psi>)\<close>
+  by (rule AOT_model_axiomI)
+     (simp add: AOT_sem_box AOT_sem_imp)
+AOT_axiom qml_2: \<open>\<box>\<phi> \<rightarrow> \<phi>\<close>
+  by (rule AOT_model_axiomI)
+     (simp add: AOT_sem_box AOT_sem_imp)
+AOT_axiom qml_3: \<open>\<diamond>\<phi> \<rightarrow> \<box>\<diamond>\<phi>\<close>
+  by (rule AOT_model_axiomI)
+     (simp add: AOT_sem_box AOT_sem_dia AOT_sem_imp)
 
-AOT_theorem qml_4: \<open>\<diamond>\<exists>x (E!x & \<not>\<^bold>\<A>E!x)\<close>
+AOT_axiom qml_4: \<open>\<diamond>\<exists>x (E!x & \<not>\<^bold>\<A>E!x)\<close>
+  apply (rule AOT_model_axiomI)
   using AOT_sem_concrete AOT_model_contingent
   by (auto simp: AOT_sem_box AOT_sem_dia AOT_sem_imp AOT_sem_exists AOT_sem_denotes
                  AOT_sem_conj AOT_sem_not AOT_sem_act AOT_sem_exe)
 
-AOT_theorem qml_act_1: \<open>\<^bold>\<A>\<phi> \<rightarrow> \<box>\<^bold>\<A>\<phi>\<close>
-  by (simp add: AOT_sem_act AOT_sem_box AOT_sem_imp)
-AOT_theorem qml_act_2: \<open>\<box>\<phi> \<equiv> \<^bold>\<A>\<box>\<phi>\<close>
-  by (simp add: AOT_sem_act AOT_sem_box AOT_sem_equiv)
+AOT_axiom qml_act_1: \<open>\<^bold>\<A>\<phi> \<rightarrow> \<box>\<^bold>\<A>\<phi>\<close>
+  by (rule AOT_model_axiomI)
+     (simp add: AOT_sem_act AOT_sem_box AOT_sem_imp)
+AOT_axiom qml_act_2: \<open>\<box>\<phi> \<equiv> \<^bold>\<A>\<box>\<phi>\<close>
+  by (rule AOT_model_axiomI)
+     (simp add: AOT_sem_act AOT_sem_box AOT_sem_equiv)
 
-AOT_theorem descriptions: \<open>x = \<^bold>\<iota>x(\<phi>{x}) \<equiv> \<forall>z(\<^bold>\<A>\<phi>{z} \<equiv> z = x)\<close>
-  by (induct; simp add: AOT_sem_equiv AOT_sem_forall AOT_sem_act AOT_sem_eq)
-     (metis (no_types, hide_lams) AOT_sem_desc_denotes AOT_sem_desc_prop AOT_sem_denotes)
+AOT_axiom descriptions: \<open>x = \<^bold>\<iota>x(\<phi>{x}) \<equiv> \<forall>z(\<^bold>\<A>\<phi>{z} \<equiv> z = x)\<close>
+proof (rule AOT_model_axiomI)
+  AOT_modally_strict {
+    AOT_show \<open>x = \<^bold>\<iota>x(\<phi>{x}) \<equiv> \<forall>z(\<^bold>\<A>\<phi>{z} \<equiv> z = x)\<close>
+      by (induct; simp add: AOT_sem_equiv AOT_sem_forall AOT_sem_act AOT_sem_eq)
+        (metis (no_types, hide_lams) AOT_sem_desc_denotes AOT_sem_desc_prop AOT_sem_denotes)
+  }
+qed
 
-AOT_theorem lambda_predicates_1: \<open>[\<lambda>\<nu>\<^sub>1...\<nu>\<^sub>n \<phi>{\<nu>\<^sub>1...\<nu>\<^sub>n}]\<down> \<rightarrow> [\<lambda>\<nu>\<^sub>1...\<nu>\<^sub>n \<phi>{\<nu>\<^sub>1...\<nu>\<^sub>n}] = [\<lambda>\<mu>\<^sub>1...\<mu>\<^sub>n \<phi>{\<mu>\<^sub>1...\<mu>\<^sub>n}]\<close>
-  by (simp add: AOT_sem_denotes AOT_sem_eq AOT_sem_imp)
-AOT_theorem lambda_predicates_1_b: \<open>[\<lambda> p]\<down> \<rightarrow> [\<lambda> p] = [\<lambda> p]\<close>
-  by (simp add: AOT_sem_denotes AOT_sem_eq AOT_sem_imp)
-AOT_theorem lambda_predicates_2: \<open>[\<lambda>x\<^sub>1...x\<^sub>n \<phi>{x\<^sub>1...x\<^sub>n}]\<down> \<rightarrow> ([\<lambda>x\<^sub>1...x\<^sub>n \<phi>{x\<^sub>1...x\<^sub>n}]x\<^sub>1...x\<^sub>n \<equiv> \<phi>{x\<^sub>1...x\<^sub>n})\<close>
-  by induct (simp add: AOT_sem_denotes AOT_sem_equiv AOT_sem_imp AOT_sem_lambda_beta)
-AOT_theorem lambda_predicates_3: \<open>[\<lambda>\<nu>\<^sub>1...\<nu>\<^sub>n [F]\<nu>\<^sub>1...\<nu>\<^sub>n] = F\<close>
-  by induct (simp add: AOT_sem_denotes AOT_sem_lambda_eta AOT_sem_vars_denote)
-AOT_theorem lambda_predicates_3_b: \<open>[\<lambda> p] = p\<close>
-  by induct (simp add: AOT_sem_eq AOT_sem_lambda0)
-AOT_theorem safe_ext: \<open>([\<lambda>\<nu>\<^sub>1...\<nu>\<^sub>n \<phi>{\<nu>\<^sub>1...\<nu>\<^sub>n}]\<down> & \<box>\<forall>\<nu>\<^sub>1...\<forall>\<nu>\<^sub>n (\<phi>{\<nu>\<^sub>1...\<nu>\<^sub>n} \<equiv> \<psi>{\<nu>\<^sub>1...\<nu>\<^sub>n})) \<rightarrow> [\<lambda>\<nu>\<^sub>1...\<nu>\<^sub>n \<psi>{\<nu>\<^sub>1...\<nu>\<^sub>n}]\<down>\<close>
+AOT_axiom lambda_predicates_1: \<open>[\<lambda>\<nu>\<^sub>1...\<nu>\<^sub>n \<phi>{\<nu>\<^sub>1...\<nu>\<^sub>n}]\<down> \<rightarrow> [\<lambda>\<nu>\<^sub>1...\<nu>\<^sub>n \<phi>{\<nu>\<^sub>1...\<nu>\<^sub>n}] = [\<lambda>\<mu>\<^sub>1...\<mu>\<^sub>n \<phi>{\<mu>\<^sub>1...\<mu>\<^sub>n}]\<close>
+  by (rule AOT_model_axiomI)
+     (simp add: AOT_sem_denotes AOT_sem_eq AOT_sem_imp)
+AOT_axiom lambda_predicates_1_b: \<open>[\<lambda> p]\<down> \<rightarrow> [\<lambda> p] = [\<lambda> p]\<close>
+  by (rule AOT_model_axiomI)
+     (simp add: AOT_sem_denotes AOT_sem_eq AOT_sem_imp)
+AOT_axiom lambda_predicates_2: \<open>[\<lambda>x\<^sub>1...x\<^sub>n \<phi>{x\<^sub>1...x\<^sub>n}]\<down> \<rightarrow> ([\<lambda>x\<^sub>1...x\<^sub>n \<phi>{x\<^sub>1...x\<^sub>n}]x\<^sub>1...x\<^sub>n \<equiv> \<phi>{x\<^sub>1...x\<^sub>n})\<close>
+proof (rule AOT_model_axiomI)
+  AOT_modally_strict {
+    AOT_show \<open>[\<lambda>x\<^sub>1...x\<^sub>n \<phi>{x\<^sub>1...x\<^sub>n}]\<down> \<rightarrow> ([\<lambda>x\<^sub>1...x\<^sub>n \<phi>{x\<^sub>1...x\<^sub>n}]x\<^sub>1...x\<^sub>n \<equiv> \<phi>{x\<^sub>1...x\<^sub>n})\<close>
+      by induct (simp add: AOT_sem_denotes AOT_sem_equiv AOT_sem_imp AOT_sem_lambda_beta)
+  }
+qed
+AOT_axiom lambda_predicates_3: \<open>[\<lambda>\<nu>\<^sub>1...\<nu>\<^sub>n [F]\<nu>\<^sub>1...\<nu>\<^sub>n] = F\<close>
+proof (rule AOT_model_axiomI)
+  AOT_modally_strict {
+    AOT_show \<open>[\<lambda>\<nu>\<^sub>1...\<nu>\<^sub>n [F]\<nu>\<^sub>1...\<nu>\<^sub>n] = F\<close>
+      by induct (simp add: AOT_sem_denotes AOT_sem_lambda_eta AOT_sem_vars_denote)
+  }
+qed
+AOT_axiom lambda_predicates_3_b: \<open>[\<lambda> p] = p\<close>
+proof (rule AOT_model_axiomI)
+  AOT_modally_strict {
+    AOT_show \<open>[\<lambda> p] = p\<close>
+      by induct (simp add: AOT_sem_eq AOT_sem_lambda0)
+  }
+qed
+AOT_axiom safe_ext: \<open>([\<lambda>\<nu>\<^sub>1...\<nu>\<^sub>n \<phi>{\<nu>\<^sub>1...\<nu>\<^sub>n}]\<down> & \<box>\<forall>\<nu>\<^sub>1...\<forall>\<nu>\<^sub>n (\<phi>{\<nu>\<^sub>1...\<nu>\<^sub>n} \<equiv> \<psi>{\<nu>\<^sub>1...\<nu>\<^sub>n})) \<rightarrow> [\<lambda>\<nu>\<^sub>1...\<nu>\<^sub>n \<psi>{\<nu>\<^sub>1...\<nu>\<^sub>n}]\<down>\<close>
+  apply (rule AOT_model_axiomI)
   using AOT_sem_lambda_coex 
   by (simp add: AOT_sem_imp AOT_sem_denotes AOT_sem_conj AOT_sem_equiv AOT_sem_box AOT_sem_forall) blast
 
-AOT_theorem nary_encoding_2: \<open>xy[F] \<equiv> x[\<lambda>\<nu> [F]\<nu>y] & y[\<lambda>\<nu> [F]x\<nu>]\<close>
-  by (simp add: AOT_sem_conj AOT_sem_equiv AOT_enc_prod_def AOT_proj_enc_prod_def
+AOT_axiom nary_encoding_2: \<open>xy[F] \<equiv> x[\<lambda>\<nu> [F]\<nu>y] & y[\<lambda>\<nu> [F]x\<nu>]\<close>
+  by (rule AOT_model_axiomI)
+     (simp add: AOT_sem_conj AOT_sem_equiv AOT_enc_prod_def AOT_proj_enc_prod_def
                 AOT_sem_unary_proj_enc AOT_sem_vars_denote)
-AOT_theorem nary_encoding_3: \<open>xyz[F] \<equiv> x[\<lambda>\<nu> [F]\<nu>yz] & y[\<lambda>\<nu> [F]x\<nu>z] & z[\<lambda>\<nu> [F]xy\<nu>]\<close>
-  by (simp add: AOT_sem_conj AOT_sem_equiv AOT_enc_prod_def AOT_proj_enc_prod_def
+AOT_axiom nary_encoding_3: \<open>xyz[F] \<equiv> x[\<lambda>\<nu> [F]\<nu>yz] & y[\<lambda>\<nu> [F]x\<nu>z] & z[\<lambda>\<nu> [F]xy\<nu>]\<close>
+  by (rule AOT_model_axiomI)
+     (simp add: AOT_sem_conj AOT_sem_equiv AOT_enc_prod_def AOT_proj_enc_prod_def
                 AOT_sem_unary_proj_enc AOT_sem_vars_denote)
-AOT_theorem nary_encoding_4: \<open>x\<^sub>1x\<^sub>2x\<^sub>3x\<^sub>4[F] \<equiv> x\<^sub>1[\<lambda>\<nu> [F]\<nu>x\<^sub>2x\<^sub>3x\<^sub>4] & x\<^sub>2[\<lambda>\<nu> [F]x\<^sub>1\<nu>x\<^sub>3x\<^sub>4] &
+AOT_axiom nary_encoding_4: \<open>x\<^sub>1x\<^sub>2x\<^sub>3x\<^sub>4[F] \<equiv> x\<^sub>1[\<lambda>\<nu> [F]\<nu>x\<^sub>2x\<^sub>3x\<^sub>4] & x\<^sub>2[\<lambda>\<nu> [F]x\<^sub>1\<nu>x\<^sub>3x\<^sub>4] &
                                            x\<^sub>3[\<lambda>\<nu> [F]x\<^sub>1x\<^sub>2\<nu>x\<^sub>4] & x\<^sub>4[\<lambda>\<nu> [F]x\<^sub>1x\<^sub>2x\<^sub>3\<nu>]\<close>
-  by (simp add: AOT_sem_conj AOT_sem_equiv AOT_enc_prod_def AOT_proj_enc_prod_def
+  by (rule AOT_model_axiomI)
+     (simp add: AOT_sem_conj AOT_sem_equiv AOT_enc_prod_def AOT_proj_enc_prod_def
                 AOT_sem_unary_proj_enc AOT_sem_vars_denote)
 
-AOT_theorem encoding: \<open>x[F] \<rightarrow> \<box>x[F]\<close>
+AOT_axiom encoding: \<open>x[F] \<rightarrow> \<box>x[F]\<close>
+  apply (rule AOT_model_axiomI)
   using AOT_sem_enc_nec 
   by (simp add: AOT_sem_imp AOT_sem_box) blast
 
-AOT_theorem nocoder: \<open>O!x \<rightarrow> \<not>\<exists>F x[F]\<close>
+AOT_axiom nocoder: \<open>O!x \<rightarrow> \<not>\<exists>F x[F]\<close>
+  apply (rule AOT_model_axiomI)
   by (simp add: AOT_sem_imp AOT_sem_not AOT_sem_exists AOT_sem_ordinary AOT_sem_dia
                 AOT_sem_lambda_beta[OF AOT_sem_ordinary_def_denotes,
                                      OF AOT_sem_vars_denote])
      (metis AOT_sem_nocoder)
 
-AOT_theorem a_objects: \<open>\<exists>x (A!x & \<forall>F(x[F] \<equiv> \<phi>{F}))\<close>
-proof -
-  AOT_obtain \<kappa> where \<open>\<kappa>\<down> & \<box>\<not>E!\<kappa> & \<forall>F (\<kappa>[F] \<equiv> \<phi>{F})\<close>
-    using AOT_sem_a_objects[of _ \<phi>]
-    by (auto simp: AOT_sem_imp AOT_sem_box AOT_sem_forall AOT_sem_exists AOT_sem_conj
-                   AOT_sem_not AOT_sem_dia AOT_sem_denotes AOT_sem_equiv) blast
-  thus ?thesis
-    unfolding AOT_sem_exists
-    by (rule_tac x=\<kappa> in exI)
-       (auto simp: AOT_sem_lambda_beta[OF AOT_sem_abstract_def_denotes]
-                   AOT_sem_box AOT_sem_dia AOT_sem_not AOT_sem_denotes AOT_var_of_term_inverse
-                   AOT_sem_equiv AOT_sem_forall AOT_sem_conj AOT_sem_abstract)
+AOT_axiom a_objects: \<open>\<exists>x (A!x & \<forall>F(x[F] \<equiv> \<phi>{F}))\<close>
+proof(rule AOT_model_axiomI)
+  AOT_modally_strict {
+    AOT_obtain \<kappa> where \<open>\<kappa>\<down> & \<box>\<not>E!\<kappa> & \<forall>F (\<kappa>[F] \<equiv> \<phi>{F})\<close>
+      using AOT_sem_a_objects[of _ \<phi>]
+      by (auto simp: AOT_sem_imp AOT_sem_box AOT_sem_forall AOT_sem_exists AOT_sem_conj
+                     AOT_sem_not AOT_sem_dia AOT_sem_denotes AOT_sem_equiv) blast
+    AOT_thus \<open>\<exists>x (A!x & \<forall>F(x[F] \<equiv> \<phi>{F}))\<close>
+      unfolding AOT_sem_exists
+      by (rule_tac x=\<kappa> in exI)
+         (auto simp: AOT_sem_lambda_beta[OF AOT_sem_abstract_def_denotes]
+                     AOT_sem_box AOT_sem_dia AOT_sem_not AOT_sem_denotes AOT_var_of_term_inverse
+                     AOT_sem_equiv AOT_sem_forall AOT_sem_conj AOT_sem_abstract)
+  }
 qed
+
+AOT_theorem universal_closure: assumes \<open>for arbitrary \<alpha>: \<phi>{\<alpha>} \<in> \<Lambda>\<^sub>\<box>\<close> shows \<open>\<forall>\<alpha> \<phi>{\<alpha>} \<in> \<Lambda>\<^sub>\<box>\<close>
+  using assms
+  by (metis AOT_term_of_var_cases AOT_model_axiom_def AOT_sem_denotes AOT_sem_forall)
+
+AOT_theorem act_closure: assumes \<open>\<phi> \<in> \<Lambda>\<^sub>\<box>\<close> shows \<open>\<^bold>\<A>\<phi> \<in> \<Lambda>\<^sub>\<box>\<close>
+  using assms by (simp add: AOT_model_axiom_def AOT_sem_act)
+
+AOT_theorem nec_closure: assumes \<open>\<phi> \<in> \<Lambda>\<^sub>\<box>\<close> shows \<open>\<box>\<phi> \<in> \<Lambda>\<^sub>\<box>\<close>
+  using assms by (simp add: AOT_model_axiom_def AOT_sem_box)
+
+AOT_theorem universal_closure_act: assumes \<open>for arbitrary \<alpha>: \<phi>{\<alpha>} \<in> \<Lambda>\<close> shows \<open>\<forall>\<alpha> \<phi>{\<alpha>} \<in> \<Lambda>\<close>
+  using assms
+  by (metis AOT_term_of_var_cases AOT_model_act_axiom_def AOT_sem_denotes AOT_sem_forall)
+
+AOT_theorem act_closure_act: assumes \<open>\<phi> \<in> \<Lambda>\<close> shows \<open>\<^bold>\<A>\<phi> \<in> \<Lambda>\<close>
+  using assms by (simp add: AOT_model_act_axiom_def AOT_sem_act)
 
 end
